Fix constant propagation.

theories/ValueOpts/ConstantPropagation.v
@@ -131,25 +131,46 @@ Inductive cp_sound : onv aval
 | CPReturn AE Cp e
   : cp_sound AE Cp (stmtReturn e)
 | CPLet AE Cp F t
-  : cp_sound AE (List.map (fun Zs => (fst Zs,lookup_list AE (fst Zs))) F ++ Cp) t
-  -> cp_sound AE Cp (stmtFun F t).
+  : (forall n Zs, get F n Zs
+             -> cp_sound AE (List.map (fun Zs => (fst Zs,lookup_list AE (fst Zs))) F ++ Cp) (snd Zs))
+    -> cp_sound AE (List.map (fun Zs => (fst Zs,lookup_list AE (fst Zs))) F ++ Cp) t
+    -> cp_sound AE Cp (stmtFun F t).
+
+Definition indexwise_R1 {A} (P:A->Prop) LA :=
+forall n a, get LA n a -> P a.
+
+Definition indexwise_R1_dec {A} {P:A->Prop} LA (Rdec:(forall n a, get LA n a -> Computable (P a)))
+      : Computable (indexwise_R1 P LA).
+unfold Computable. revert LA Rdec. fix 1. intros LA Rdec.
+destruct LA; try now left; isabsurd.
+intros. destruct (Rdec 0 a).
+- eauto using get.
+- destruct (indexwise_R1_dec LA); clear indexwise_R1_dec; eauto using get.
+  + left. hnf; intros. inv H; eauto.
+  + right; intro HH. eapply n; hnf; intros; eapply HH; eauto using get.
+- right; intro HH. eapply n; hnf; intros; eapply HH; eauto using get.
+Defined.
 
 Instance cp_sound_dec AE ZL s : Computable (cp_sound AE ZL s).
 Proof.
-  hnf. general induction s; try dec_solve.
-  - edestruct IHs; decide (Some (exp_eval AE e) = AE x); dec_solve.
+  hnf. revert AE ZL; sind s; intros; destruct s; try dec_solve.
+  - edestruct (IH s); eauto; decide (Some (exp_eval AE e) = AE x); try dec_solve.
   - decide (aval2bool (op_eval AE e) = Some false);
     decide (aval2bool (op_eval AE e) = Some true).
     + unfold val_false, val_true in *. congruence.
-    + edestruct IHs2; try dec_solve.
-    + edestruct IHs1; try dec_solve.
-    + edestruct IHs1; edestruct IHs2; try dec_solve.
+    + edestruct (IH s2 ltac:(eauto) (update_cond AE e false) ZL); eauto; try dec_solve.
+    + edestruct (IH s1 ltac:(eauto) (update_cond AE e true) ZL); eauto; dec_solve.
+    + edestruct (IH s1 ltac:(eauto) (update_cond AE e true) ZL);
+        edestruct (IH s2 ltac:(eauto) (update_cond AE e false) ZL); eauto; try dec_solve.
   - destruct (get_dec ZL (counted l)) as [[[]]|]; try dec_solve.
     decide (length l0 = length Y); try dec_solve.
     decide (PIR2 le_precise l1 (List.map (op_eval AE ∘ Some) Y));
       try dec_solve.
-  - edestruct (IHs s1 AE (List.map (fun Zs => (fst Zs,lookup_list AE (fst Zs))) F ++ ZL));
-    edestruct (IHs2 AE ((Z,lookup_list AE Z)::ZL)); try dec_solve.
+  - assert (SZ:size s < size (stmtFun F s)) by eauto.
+    edestruct (IH s SZ AE (List.map (fun Zs => (fst Zs,lookup_list AE (fst Zs))) F ++ ZL)).
+    exploit (@indexwise_R1_dec _ (fun Zs => cp_sound AE ((fun Zs0 : params * stmt => (fst Zs0, lookup_list AE (fst Zs0))) ⊝ F ++ ZL) (snd Zs)) F); eauto.
+    intros. eapply IH; eauto. destruct H.
+    dec_solve. dec_solve. dec_solve.
 Defined.
 
 Definition cp_eqn (E:onv aval) x :=
@@ -157,6 +178,14 @@ Definition cp_eqn (E:onv aval) x :=
     | Some (wTA c) => singleton (EqnEq (Var x) (Con c))
     | _ => ∅
   end.
+
+Instance cp_eqn_eq E
+  : Proper (_eq ==> _eq) (cp_eqn E).
+Proof.
+  unfold Proper, respectful, cp_eqn; intros; subst.
+  hnf in H; subst.
+  cases; eauto.
+Qed.
 
 Definition cp_eqns (E:onv aval) (lv:set var) : eqns :=
   fold union (map (cp_eqn E) lv) ∅.
@@ -213,8 +242,8 @@ Lemma cp_eqns_agree lv E E'
   -> cp_eqns E lv [=] cp_eqns E' lv.
 Proof.
   intros. hnf; intro. unfold cp_eqns.
-  rewrite map_agree; eauto using cp_eqn_agree. reflexivity.
-  intuition. intuition.
+  setoid_rewrite map_agree; try eapply cp_eqn_eq; try reflexivity.
+  eapply cp_eqn_agree. symmetry; eauto.
 Qed.
 
 Inductive same_shape (A B:Type) : ann B -> ann A -> Prop :=
@@ -247,29 +276,30 @@ Lemma zip2Ann_get X Y Z f a b
 Definition cp_eqns_ann (a:ann (onv aval)) (b:ann (set var)) : ann eqns :=
   zip2Ann cp_eqns a b (ann0 ∅).
 
-Definition cp_choose_exp E e :=
-  match exp_eval E e with
+Definition cp_choose_op E e :=
+  match op_eval E e with
     | wTA c => Con c
     | _ => e
   end.
 
 
-Fixpoint constantPropagate (AE:onv aval) s : stmt :=
+Fixpoint constantPropagate (AE:onv aval) s {struct s} : stmt :=
   match s with
-    | stmtLet x e s =>
-      stmtLet x (cp_choose_exp AE e) (constantPropagate AE s)
+    | stmtLet x (Operation e) s =>
+      stmtLet x (Operation (cp_choose_op AE e)) (constantPropagate AE s)
+    | stmtLet x (Call f Y) s =>
+      stmtLet x (Call f (List.map (cp_choose_op AE) Y))
+              (constantPropagate AE s)
     | stmtIf e s t =>
-      stmtIf (cp_choose_exp AE e)
+      stmtIf (cp_choose_op AE e)
              (constantPropagate (update_cond AE e true) s)
              (constantPropagate (update_cond AE e false) t)
     | stmtApp f Y =>
-      stmtApp f (List.map (cp_choose_exp AE) Y)
-    | stmtReturn e => stmtReturn (cp_choose_exp AE e)
-    | stmtExtern x f Y s =>
-      stmtExtern x f (List.map (cp_choose_exp AE) Y)
-                 (constantPropagate AE s)
-    | stmtFun Z s t =>
-      stmtFun Z (constantPropagate AE s) (constantPropagate AE t)
+      stmtApp f (List.map (cp_choose_op AE) Y)
+    | stmtReturn e => stmtReturn (cp_choose_op AE e)
+    | stmtFun F t =>
+      stmtFun (List.map (fun Zs => (fst Zs, constantPropagate AE (snd Zs))) F)
+              (constantPropagate AE t)
   end.
 
 Lemma zip2Ann_get X Y Z (f:X->Y->Z) a b z
@@ -285,9 +315,8 @@ Lemma in_or_not X `{OrderedType X} x s
   + { x ∉ s /\ s [=] s \ {{x}} }.
 Proof.
   decide (x ∈ s); [left|right]; split; eauto.
-  - cset_tac; intuition. decide (_eq a x); eauto.
-    rewrite <- H1; eauto.
-  - cset_tac; intuition.
+  - cset_tac.
+  - cset_tac.
 Qed.
 
 Lemma in_cp_eqns AE x lv v
@@ -311,10 +340,10 @@ Lemma cp_eqns_satisfies_env AE E x v lv
   -> satisfiesAll E (cp_eqns AE lv)
   -> E x = ⎣v ⎦.
 Proof.
-  intros. exploit H1; eauto.
+  intros. exploit H1 as SAT; eauto.
   instantiate (1:=EqnEq (Var x) (Con v)).
   eapply in_cp_eqns; eauto.
-  hnf in X; simpl in *. inv X; eauto.
+  hnf in SAT; simpl in *. inv SAT; eauto.
 Qed.
 
 Ltac smatch :=
@@ -334,17 +363,17 @@ Ltac dmatch :=
 
 Ltac imatch := dmatch; smatch; isabsurd.
 
-Lemma exp_eval_same e lv AE E v
-:   Exp.freeVars e ⊆ lv
-    -> exp_eval AE e = wTA v
+Lemma op_eval_same e lv AE E v
+:   Op.freeVars e ⊆ lv
+    -> op_eval AE e = wTA v
     -> satisfiesAll E (cp_eqns AE lv)
-    -> exists v', Exp.exp_eval E e = Some v' /\ option_eq eq ⎣v' ⎦ ⎣v ⎦.
+    -> exists v', Op.op_eval E e = Some v' /\ option_eq eq ⎣v' ⎦ ⎣v ⎦.
 Proof.
   intros. general induction e; simpl in * |- *; eauto 20 using @option_eq.
   - exploit cp_eqns_satisfies_env; eauto.
-    + rewrite <- H. cset_tac; eauto.
-    + destruct (AE v). f_equal; eauto. congruence.
-    + eexists v0; eauto using @option_eq.
+    + rewrite <- H. cset_tac.
+    + destruct (AE n). f_equal; eauto. congruence.
+    + eexists v; eauto using @option_eq.
   - repeat imatch.
     edestruct IHe; eauto; dcr.
     rewrite H5; simpl.
@@ -360,21 +389,23 @@ Proof.
     eexists v; split; eauto using @option_eq.
 Qed.
 
-Lemma exp_eval_entails AE e v x lv
-: Exp.freeVars e ⊆ lv
-  -> exp_eval AE e = wTA v
-  -> entails ({EqnEq (Var x) e ; { EqnEq (Var x) (cp_choose_exp AE e) ;
+Lemma op_eval_entails AE e v x lv
+: Op.freeVars e ⊆ lv
+  -> op_eval AE e = wTA v
+  -> entails ({EqnEq (Var x) e ; { EqnEq (Var x) (cp_choose_op AE e) ;
                                      cp_eqns AE lv } }) (singleton (EqnEq (Var x) (Con v))).
 Proof.
   intros.
   unfold entails; intros. unfold satisfiesAll; intros.
   exploit (H1 (EqnEq (Var x) e)); eauto.
-  cset_tac; intuition. cset_tac. invc H2; simpl in *; subst; simpl.
-  eapply satisfiesAll_add in H1; dcr.
-  eapply satisfiesAll_add in H3; dcr.
-  edestruct exp_eval_same; try eapply H0; eauto; dcr.
-  unfold cp_choose_exp in *; simpl in *.
-  rewrite H0 in H1. eauto.
+  - cset_tac.
+  - cset_tac'.
+    invc H2; simpl in *; subst; simpl.
+    eapply satisfiesAll_add in H1; dcr.
+    eapply satisfiesAll_add in H4; dcr.
+    edestruct op_eval_same; try eapply H0; eauto; dcr.
+    unfold cp_choose_op in *; simpl in *.
+    rewrite H0 in H1. eauto.
 Qed.
 
 Lemma cp_eqns_single AE x
@@ -389,24 +420,23 @@ Proof.
   eapply transpose_union.
 Qed.
 
-
 Lemma cp_choose_approx AE e lv
-: Exp.freeVars e ⊆ lv
-  -> entails (cp_eqns AE lv) {EqnApx e (cp_choose_exp AE e)}.
+: Op.freeVars e ⊆ lv
+  -> entails (cp_eqns AE lv) {EqnApx e (cp_choose_op AE e)}.
 Proof.
-  unfold cp_choose_exp. case_eq (exp_eval AE e); intros.
+  unfold cp_choose_op. case_eq (op_eval AE e); intros.
   - eapply entails_eqns_apx_refl.
   - hnf; intros.
-    case_eq (Exp.exp_eval E e); intros; simpl.
-    + edestruct exp_eval_same; try eapply H1; eauto; dcr.
-      hnf; intros. cset_tac. rewrite <- H3; simpl.
+    case_eq (Op.op_eval E e); intros; simpl.
+    + edestruct op_eval_same; try eapply H1; eauto; dcr.
+      hnf; intros. cset_tac'. rewrite <- H3; simpl.
       rewrite H4. inv H5. reflexivity.
-    + edestruct exp_eval_same; try eapply H1; eauto; dcr. congruence.
+    + edestruct op_eval_same; try eapply H1; eauto; dcr. congruence.
 Qed.
 
 Lemma cp_choose_approx_list AE Y lv
-: list_union (List.map Exp.freeVars Y) ⊆ lv
-  ->  entails (cp_eqns AE lv) (list_EqnApx Y (List.map (cp_choose_exp AE) Y)).
+: list_union (List.map Op.freeVars Y) ⊆ lv
+  ->  entails (cp_eqns AE lv) (list_EqnApx Y (List.map (cp_choose_op AE) Y)).
 Proof.
   intros. general induction Y; simpl.
   - unfold list_EqnApx. simpl. eapply entails_empty.
@@ -421,27 +451,28 @@ Proof.
 Qed.
 
 Lemma cp_choose_exp_freeVars AE e D
-: Exp.freeVars e ⊆ D
-  -> Exp.freeVars (cp_choose_exp AE e) ⊆ D.
+: Op.freeVars e ⊆ D
+  -> Op.freeVars (cp_choose_op AE e) ⊆ D.
 Proof.
   intros.
-  unfold cp_choose_exp. case_eq (exp_eval AE e); intros; eauto using incl_empty.
+  unfold cp_choose_op.
+  case_eq (op_eval AE e); intros; eauto using incl_empty.
 Qed.
 
 Lemma cp_choose_exp_live_sound_exp AE e lv
-:  Exp.freeVars e ⊆ lv
-   -> Exp.freeVars (cp_choose_exp AE e) ⊆ lv.
+:  Op.freeVars e ⊆ lv
+   -> Op.freeVars (cp_choose_op AE e) ⊆ lv.
 Proof.
-  intros. unfold cp_choose_exp.
-  destruct (exp_eval AE e); intros; eauto.
+  intros. unfold cp_choose_op.
+  destruct (op_eval AE e); intros; eauto.
   simpl; eapply incl_empty.
 Qed.
 
 Lemma cp_choose_exp_eval_exp AE e v
-: exp_eval AE e = wTA v
-  -> exp_eval AE (cp_choose_exp AE e) = wTA v.
+: op_eval AE e = wTA v
+  -> op_eval AE (cp_choose_op AE e) = wTA v.
 Proof.
-  intros. unfold cp_choose_exp. rewrite H; eauto.
+  intros. unfold cp_choose_op. rewrite H; eauto.
 Qed.
 
 Lemma subst_eqns_in gamma ϱ Gamma
@@ -478,18 +509,16 @@ Lemma cp_eqns_freeVars AE lv
 Proof.
   hnf; intros.
   eapply incl_fold_union in H; destruct H; isabsurd.
-  destruct H; dcr.
-  eapply map_iff in H0; destruct H0; dcr; intuition.
-  eapply cp_eqns_in in H0. destruct H0; dcr.
-  eapply H2 in H1.
-  unfold cp_eqn in H3.
+  destruct H; dcr. cset_tac'.
+  eapply cp_eqns_in in H. cset_tac'.
+  unfold cp_eqn in H4.
   case_eq (AE x1); intros.
-  - rewrite H in H3.
+  - rewrite H in *.
     destruct a0.
     + isabsurd.
-    + cset_tac. hnf in H3; subst; simpl in *.
-      cset_tac; intuition.
-  - rewrite H in H3. isabsurd.
+    + cset_tac'. hnf in H4; subst; simpl in *.
+      rewrite H0 in H1. cset_tac.
+  - rewrite H in H4. isabsurd.
 Qed.
 
 Lemma in_subst_eqns gamma Z Y AE
@@ -506,7 +535,7 @@ Proof.
   edestruct cp_eqns_in as [x ?]; eauto; dcr.
   unfold cp_eqn in H4. case_eq (AE x); intros.
   - rewrite H1 in H4. destruct a; isabsurd.
-    cset_tac. invc H4.
+    cset_tac'. invc H4.
     unfold subst_eqn; simpl.
     edestruct (update_with_list_lookup_in_list sid Z Y) as [? [? ]]; eauto; dcr.
     invc H9. invc H7.
@@ -516,8 +545,8 @@ Qed.
 
 Lemma entails_cp_eqns_subst AE D Z Y
 : length Z = length Y
-  -> PIR2 le_precise (lookup_list AE Z) (List.map (exp_eval AE ∘ Some) Y)
-  -> list_union (List.map Exp.freeVars Y)[<=]D
+  -> PIR2 le_precise (lookup_list AE Z) (List.map (op_eval AE ∘ Some) Y)
+  -> list_union (List.map Op.freeVars Y)[<=]D
   -> entails (cp_eqns AE D)
             (subst_eqns (sid [Z <-- Y]) (cp_eqns AE (of_list Z))).
 Proof.
@@ -525,38 +554,37 @@ Proof.
   hnf. intros. hnf. intros.
 
   edestruct in_subst_eqns as [? [? []]]; eauto; dcr.
-  edestruct PIR2_nth_2; eauto. eapply map_get_1; eauto. dcr.
+  edestruct PIR2_nth_2; eauto; dcr.
   exploit lookup_list_get; eauto. subst.
   inversion H7; try congruence.
-  edestruct exp_eval_same; eauto; dcr.
-  rewrite <- INCL.
-  eapply incl_list_union. eapply map_get_1; eauto. reflexivity.
-  simpl. rewrite H9.
-  econstructor. inv H10. congruence.
+  edestruct op_eval_same; eauto; dcr.
+  - rewrite <- INCL.
+    eapply incl_list_union. eapply map_get_1; eauto. reflexivity.
+  - simpl. rewrite H9.
+    econstructor. inv H10. congruence.
 Qed.
 
 
 Lemma entails_cp_eqns_subst_choose AE AE' D Z Y
 : length Z = length Y
-  -> PIR2 le_precise (lookup_list AE' Z) (List.map (exp_eval AE ∘ Some) Y)
-  -> list_union (List.map Exp.freeVars Y)[<=]D
+  -> PIR2 le_precise (lookup_list AE' Z) (List.map (op_eval AE ∘ Some) Y)
+  -> list_union (List.map Op.freeVars Y)[<=]D
   -> entails (cp_eqns AE D)
-            (subst_eqns (sid [Z <-- List.map (cp_choose_exp AE) Y]) (cp_eqns AE' (of_list Z))).
+            (subst_eqns (sid [Z <-- List.map (cp_choose_op AE) Y]) (cp_eqns AE' (of_list Z))).
 Proof.
   intros LEQ le_prec INCL.
   hnf. intros. hnf. intros.
 
-  edestruct in_subst_eqns as [? [? []]]; try eapply H0; eauto; dcr.
-  rewrite map_length; eauto.
+  edestruct in_subst_eqns as [? [? []]]; try eapply H0; eauto; dcr; subst.
   edestruct map_get_4; eauto; dcr.
-  edestruct PIR2_nth_2; eauto. eapply map_get_1; eauto. dcr.
+  edestruct PIR2_nth_2; eauto; dcr.
   exploit lookup_list_get; eauto. subst.
-  inversion H9; try congruence.
-  edestruct exp_eval_same; eauto; dcr.
+  inversion H8; try congruence.
+  edestruct op_eval_same; eauto; dcr.
   rewrite <- INCL.
   eapply incl_list_union. eapply map_get_1; eauto. reflexivity.
-  hnf; simpl.
-  rewrite <- H5. unfold cp_choose_exp. rewrite <- H10. simpl.
+  hnf; simpl. inv_get.
+  rewrite H6. unfold cp_choose_op. rewrite <- H10. simpl.
   constructor. inv H12. congruence.
 Qed.
 
@@ -566,7 +594,7 @@ Lemma cp_eqns_update D x c AE
 Proof.
   intros.
   assert (D [=] {{x}} ∪ (D \ {{x}})). {
-    cset_tac; intuition. decide (a = x); subst; intuition. inv H2; eauto.
+    cset_tac.
   }
   rewrite H0 at 1. rewrite cp_eqns_union. rewrite cp_eqns_single.
   unfold cp_eqn. lud; isabsurd.
@@ -574,127 +602,219 @@ Proof.
   hnf; intros. lud. inv e0; subst. exfalso; cset_tac; intuition.
 Qed.
 
-
-Lemma cp_sound_eqn AE Cp Es s (ang:ann (set var * set var))
-: let Gamma := (cp_eqns AE (fst (getAnn ang))) in
-cp_sound AE Cp s
--> renamedApart s ang
--> labelsDefined s (length Es)
--> (forall n a aY Z, get Es n a
-              -> get Cp n (Z,aY)
-              -> (exists AE', aY = lookup_list AE' Z
-                       /\ snd a [=] cp_eqns AE' (of_list Z))
-                /\ (fst (fst (fst a))) = Z)
--> eqn_sound Es s (constantPropagate AE s) Gamma ang.
+Lemma unsat_bool_eq_val E e v
+  : (forall w, Op.op_eval E e = Some w -> bool2val (val2bool w) <> v)
+    -> ~ satisfies E (EqnEq (UnOp UnOpToBool e) (Con v)).
 Proof.
-  intro. subst Gamma.
-  intros CP SSA LD LINV.
+  intros NE SAT. hnf in SAT. simpl in *.
+  case_eq (Op.op_eval E e); intros.
+  - rewrite H in SAT; simpl in *. inv SAT.
+    eapply NE; eauto.
+  - rewrite H in SAT; isabsurd.
+Qed.
+
+Lemma aval2bool_inv_val b AE e lv (FV:Op.freeVars e [<=] lv)
+  : aval2bool (op_eval AE e) = ⎣ b ⎦
+    -> forall E, satisfiesAll E (cp_eqns AE lv) -> exists v, Op.op_eval E e = Some v /\
+             bool2val (val2bool v) = bool2val b.
+Proof.
+  intros.
+  case_eq (op_eval AE e); intros.
+  - rewrite H1 in H; eauto. isabsurd.
+  - rewrite H1 in H. inv H.
+    edestruct op_eval_same; eauto.
+    eexists x; split; eauto; dcr.
+    inv H4. reflexivity.
+Qed.
+
+Lemma satisfies_BinOpEq_inv_true E e e'
+  : satisfies E (EqnEq (UnOp UnOpToBool (BinOp BinOpEq e e')) (Con val_true))
+    -> satisfies E (EqnEq e e').
+Proof.
+  intros. hnf in H. simpl in *.
+  destruct (Op.op_eval E e); isabsurd.
+  destruct (Op.op_eval E e'); isabsurd.
+  simpl in *. inv H.
+  pose proof (Integers.Int.eq_spec v v0).
+  destruct (Integers.Int.eq v v0); intros; isabsurd.
+  subst; eauto. reflexivity.
+Qed.
+
+Lemma satisfies_UnOpToBool_inv_false E e
+  : satisfies E (EqnEq (UnOp UnOpToBool e) (Con val_false))
+    -> satisfies E (EqnEq e (Con default_val)).
+Proof.
+  intros. hnf in H. simpl in *.
+  destruct (Op.op_eval E e); isabsurd.
+  simpl in *. inv H.
+  unfold val2bool in H2. cases in H2.
+  - reflexivity.
+  - simpl in *. isabsurd.
+Qed.
+
+Lemma satisfies_single E gamma
+  : satisfies E gamma
+    -> satisfiesAll E {gamma}.
+Proof.
+  intros; hnf; intros.
+  cset_tac'. rewrite <- H0; eauto.
+Qed.
+
+Lemma satisfies_single' E gamma
+  : satisfiesAll E {gamma}
+    -> satisfies E gamma.
+Proof.
+  intros. eapply H. cset_tac.
+Qed.
+
+Lemma satisfies_add_extr E gamma Gamma
+  : satisfiesAll E {gamma; Gamma}
+    -> satisfies E gamma.
+Proof.
+  intros. eapply H. cset_tac.
+Qed.
+
+Lemma satisfies_add_drop E gamma Gamma
+  : satisfiesAll E {gamma; Gamma}
+    -> satisfiesAll E Gamma.
+Proof.
+  intros. hnf; intros. eapply H. cset_tac.
+Qed.
+
+
+Lemma cp_sound_eqn AE Cp ZL GL ΓL s (ang:ann (set var * set var))
+ (CP:cp_sound AE Cp s)
+ (RA: renamedApart s ang)
+ (LD: labelsDefined s (length ZL))
+ (Len1: ❬ZL❭ = ❬GL❭)
+ (Len2: ❬ZL❭ = ❬ΓL❭)
+ (Len3: ❬ZL❭ = ❬Cp❭)
+  (LINV:(forall n aY Z G Γ Z', get ZL n Z
+                   -> get GL n G
+                   -> get ΓL n Γ
+                   -> get Cp n (Z',aY)
+                   -> (exists AE', aY = lookup_list AE' Z
+                             /\ Γ [=] cp_eqns AE' (of_list Z)) /\ Z' = Z))
+  :  eqn_sound ZL GL ΓL s (constantPropagate AE s) (cp_eqns AE (fst (getAnn ang))) ang.
+Proof.
   general induction CP; invt renamedApart; invt labelsDefined; simpl.
-  - econstructor.
-    eapply eqn_sound_entails_monotone; eauto.
-    + rewrite H7; simpl. rewrite cp_eqns_add.
-      eapply entails_union; split.
-      unfold cp_eqn. case_eq (AE x); intros; eauto using entails_empty.
-      rewrite H0 in H.
-      destruct a; eauto using entails_empty.
-      eapply exp_eval_entails; eauto. congruence.
-      eapply entails_monotone. reflexivity.
-      cset_tac; intuition.
-    + eapply cp_choose_approx; eauto.
-    + eapply cp_choose_exp_freeVars; eauto.
+  - simpl in *.
+    destruct e.
+    + econstructor. set_simpl.
+      * eapply eqn_sound_entails_monotone; eauto.
+        pe_rewrite. rewrite cp_eqns_add.
+        eapply entails_union; split.
+        -- unfold cp_eqn.
+           case_eq (AE x); intros; eauto using entails_empty.
+           rewrite H0 in H. inv H.
+           cases; eauto using entails_empty.
+           eapply op_eval_entails; eauto.
+        -- eapply entails_monotone. reflexivity.
+           cset_tac.
+      * eapply cp_choose_approx; eauto.
+      * eapply cp_choose_exp_freeVars; eauto.
+    + econstructor. set_simpl.
+      * eapply eqn_sound_entails_monotone; eauto.
+        pe_rewrite. rewrite cp_eqns_add.
+        eapply entails_union; split.
+        -- unfold cp_eqn.
+           case_eq (AE x); intros; eauto using entails_empty.
+           rewrite H0 in H. inv H.
+           eauto using entails_empty.
+        -- reflexivity.
+      * eapply cp_choose_approx_list; eauto.
+      * simpl in *. rewrite <- H4.
+        eapply list_union_incl; eauto with cset.
+        intros; inv_get.
+        eapply cp_choose_exp_freeVars; eauto.
+        eapply incl_list_union; eauto with get.
+      * eauto with len.
   - econstructor; intros; eauto.
     + {
-        decide (aval2bool (exp_eval AE e) = Some false).
+        decide (aval2bool (op_eval AE e) = Some false).
         - eapply EqnUnsat.
-          hnf. intros. intro.
-          exploit H3. cset_tac. left. reflexivity.
-          hnf in X. simpl in *.
-          case_eq (exp_eval AE e); intros.
-          + rewrite H4 in e0; simpl in *; congruence.
-          + edestruct exp_eval_same; eauto; dcr.
-            hnf; intros. eapply H3. cset_tac. right; eauto.
-            inv H16.
-            rewrite H11 in X. rewrite H4 in e0. inv e0.
-            simpl in *.
-            unfold option_lift1, comp in X. rewrite H17 in X.
-            inv X. isabsurd.
+          eapply unsatisfiable_add_left. intros.
+          eapply unsat_bool_eq_val; intros.
+          edestruct aval2bool_inv_val; eauto; dcr.
+          assert (w = x) by congruence; subst.
+          rewrite H16. simpl. intro.
+          eapply val_true_false_neq. congruence.
         - eapply eqn_sound_entails_monotone; eauto.
-          rewrite H12; eauto. simpl.
+          pe_rewrite.
           hnf. intros. cases.
-          + inv i; simpl in *.
+          + inv COND; simpl in *.
             rewrite cp_eqns_update.
             * eapply satisfiesAll_union; split.
-              hnf; intros. cset_tac. invc H4.
-              simpl.
-              exploit H3. cset_tac. left; reflexivity.
-              case_eq (E x); intros. simpl in *.
-              rewrite H4 in X. simpl in *.
-              unfold option_lift1, comp in X.
-              cases in X; subst; try econstructor; eauto.
-              simpl in *. inv X. inv H16.
-              simpl in *. rewrite H4 in X. isabsurd.
-              hnf; intros. eapply H3. cset_tac; right; eauto.
-              eapply cp_eqns_morphism_subset; try eapply H4. eapply minus_incl.
-            * revert H6; clear_all; intros; cset_tac; intuition.
-          + hnf; intros. eapply H3. cset_tac; right; eauto.
+              -- eapply satisfies_single.
+                 eapply satisfies_BinOpEq_inv_true.
+                 eapply satisfies_add_extr; eauto.
+              -- rewrite minus_incl.
+                 eapply satisfies_add_drop; eauto.
+            * eauto with cset.
+          + eapply satisfies_add_drop; eauto.
       }
     + {
-        decide (aval2bool (exp_eval AE e) = Some true).
+        decide (aval2bool (op_eval AE e) = Some true).
         - eapply EqnUnsat.
-          hnf. intros. intro.
-          exploit H3. cset_tac. left; reflexivity.
-          simpl in *.
-          case_eq (exp_eval AE e); intros.
-          + rewrite H4 in e0; simpl in *; congruence.
-          + edestruct exp_eval_same; eauto; dcr.
-            hnf; intros. eapply H3. cset_tac; right; eauto.
-            rewrite H11 in X. inv H16.
-            rewrite H4 in e0. simpl in *. inv e0.
-            unfold option_lift1, comp in X. rewrite H17 in X.
-            inv X. isabsurd.
+          eapply unsatisfiable_add_left. intros.
+          eapply unsat_bool_eq_val; intros.
+          edestruct aval2bool_inv_val; eauto; dcr.
+          assert (w = x) by congruence; subst.
+          rewrite H16. intro. simpl in *.
+          eapply val_true_false_neq. congruence.
         - eapply eqn_sound_entails_monotone; eauto.
-          + rewrite H13; eauto. simpl.
-            cases.
-            * inv i; simpl in *.
-              rewrite cp_eqns_update.
-              hnf; intros.
-              eapply satisfiesAll_union; split.
-              hnf; intros. cset_tac. invc H4.
-              simpl. exploit H3. cset_tac. left; reflexivity.
-              simpl in *. case_eq (E v); intros.
-              rewrite H4 in X. simpl in *.
-              unfold option_lift1, comp in X.
-              destruct v0; simpl in *. constructor; eauto. inv X; isabsurd.
-              rewrite H4 in X. isabsurd.
-              hnf; intros. eapply H3. cset_tac; right; eauto.
-              eapply cp_eqns_morphism_subset; try eapply H4. eapply minus_incl.
-              revert H6; clear_all; intros; cset_tac; intuition.
-            * hnf; intros. hnf; intros. eapply H3. cset_tac; right; eauto.
+          pe_rewrite.
+          hnf. intros. cases.
+          + inv COND; simpl in *.
+            rewrite cp_eqns_update.
+            * eapply satisfiesAll_union; split.
+              -- eapply satisfies_single.
+                 eapply satisfies_UnOpToBool_inv_false.
+                 eapply satisfies_add_extr; eauto.
+              -- rewrite minus_incl.
+                 eapply satisfies_add_drop; eauto.
+            * eauto with cset.
+          + eapply satisfies_add_drop; eauto.
       }
     + eapply cp_choose_approx; eauto.
   - edestruct get_in_range as [a ?]; eauto.
-    destruct a as [[[Zb G] Γf] EqS].
-    exploit LINV; eauto; dcr; simpl in *. subst Zb.
-    econstructor; eauto.
-    + rewrite map_length; eauto.
-    + subst. rewrite H8.
+    inv_get.
+    edestruct LINV; eauto; dcr; simpl in *. subst.
+    econstructor; eauto with len.
+    + rewrite H11.
       eapply entails_cp_eqns_subst_choose; eauto.
     + eapply cp_choose_approx_list; eauto.
   - econstructor; eauto using cp_choose_approx.
-  - eapply EqnLet with (Γ2:=cp_eqns AE D) (EqS:=cp_eqns AE (of_list Z)).
+  - assert (INV:forall (n : nat) (aY : 〔؟ aval〕) (Z : params) (G : ⦃nat⦄) (Γ : ⦃eqn⦄) Z',
+               get (fst ⊝ F ++ ZL) n Z ->
+               get (tab D ‖F‖ ++ GL) n G ->
+               get ((fun '(Z1, _) => cp_eqns AE (of_list Z1)) ⊝ F ++ ΓL) n Γ ->
+               get ((fun Zs : params * stmt => (fst Zs, lookup_list AE (fst Zs))) ⊝ F ++ Cp) n (Z', aY) ->
+               (exists AE' : nat -> ؟ aval, aY = lookup_list AE' Z /\ Γ [=] cp_eqns AE' (of_list Z)) /\ Z' = Z). {
+      intros.
+      eapply get_app_cases in H1. destruct H1; dcr.
+      - inv_get. split; eauto. eexists; split; eauto.
+        destruct x; reflexivity.
+      - len_simpl.
+        rewrite get_app_ge in H11; eauto with len.
+        rewrite get_app_ge in H13; eauto with len.
+        rewrite get_app_ge in H2; eauto with len.
+    }
+    eapply EqnFun with (Γ2:=cp_eqns AE D) (ΓF:=List.map (fun '(Z,s) => cp_eqns AE (of_list Z)) F);
+      eauto with len.
+    + intros; inv_get; eauto.
+    + intros; inv_get; eauto.
+      exploit H0; eauto; eauto with len.
+      edestruct H5; eauto; dcr; eauto with len.
+      simpl in *.
+      rewrite H11 in H2. rewrite cp_eqns_union in H2.
+      eapply H2.
     + eapply eqn_sound_entails_monotone; eauto.
-      eapply IHCP1; eauto.
-      * intros; simpl.
-        inv H; inv H0; simpl; eauto.
-      * rewrite H6. simpl.
-        rewrite cp_eqns_union. reflexivity.
-    + eapply eqn_sound_entails_monotone; eauto.
-      eapply IHCP2; eauto.
-      * intros; simpl.
-        inv H; inv H0; simpl; eauto.
-      * rewrite H9; reflexivity.
-    + rewrite cp_eqns_freeVars. eapply incl_right.
-    + rewrite cp_eqns_freeVars. reflexivity.
+      * eapply IHCP; eauto; eauto with len.
+      * pe_rewrite. reflexivity.
+    + intros; inv_get; destruct Zs; simpl.
+      rewrite cp_eqns_freeVars. eapply incl_right.
+    + rewrite cp_eqns_freeVars. eauto.
     + reflexivity.
 Qed.
 
@@ -706,12 +826,17 @@ Lemma cp_eqns_no_assumption d G
    -> cp_eqns (fun x0 : var => MapInterface.find x0 d) G [=] ∅.
 Proof.
   intros. revert H. pattern G. eapply set_induction.
-  intros. eapply empty_is_empty_1 in H. rewrite H.
-  reflexivity.
-  intros. eapply Add_Equal in H1. rewrite H1.
-  assert ({x; s} [=] {{x}} ∪ s) by (cset_tac; intuition).
-  rewrite H3. rewrite cp_eqns_union.
-  rewrite cp_eqns_single. unfold cp_eqn.
-  rewrite H2. rewrite H. cset_tac; intuition. intros; eapply H2.
-  rewrite H1. cset_tac; intuition. rewrite H1. cset_tac; intuition.
+  - intros.
+    eapply empty_is_empty_1 in H. rewrite H.
+    reflexivity.
+  - intros. eapply Add_Equal in H1. rewrite H1.
+    assert ({x; s} [=] {{x}} ∪ s) by cset_tac.
+    rewrite H3. rewrite cp_eqns_union.
+    rewrite cp_eqns_single. unfold cp_eqn.
+    rewrite H2.
+    + rewrite H.
+      * cset_tac.
+      * intros; eapply H2.
+        rewrite H1. cset_tac.
+    + rewrite H1. cset_tac.
 Qed.
