theories/ValueOpts/Eqn.v
@@ -98,6 +98,15 @@ Definition eqns := set eqn.
 Definition satisfiesAll (E:onv val) (Gamma:eqns) :=
   forall gamma, gamma ∈ Gamma -> satisfies E gamma.
 
+
+Lemma satisfiesAll_monotone E Gamma Γ'
+: satisfiesAll E Gamma
+  -> Γ' ⊆ Gamma
+  -> satisfiesAll E Γ'.
+Proof.
+  intros. hnf; intros. eapply H; eauto.
+Qed.
+
 Definition freeVars (gamma:eqn) :=
   match gamma with
     | EqnEq e e' => Op.freeVars e ∪ Op.freeVars e'
@@ -110,6 +119,18 @@ Definition eqns_freeVars (Gamma:eqns) := fold union (map freeVars Gamma) ∅.
 Definition entails Gamma Γ' := forall E, satisfiesAll E Gamma -> satisfiesAll E Γ'.
 
 Definition not_entails Gamma gamma := exists E, satisfiesAll E Gamma /\ ~ satisfies E gamma.
+
+
+Lemma not_entails_antitone Gamma Γ' gamma
+: not_entails Γ' gamma
+  -> Gamma ⊆ Γ'
+  -> not_entails Gamma gamma.
+Proof.
+  intros. hnf; intros.
+  edestruct H as [E ?]; dcr.
+  eexists E; intros; split; eauto using satisfiesAll_monotone; eauto.
+Qed.
+
 
 
 Definition onvLe X (E E':onv X)
@@ -145,5 +166,669 @@ Definition subst_eqns (ϱ : env op) (G:eqns) : eqns :=
 
 Definition sid := fun x => Var x.
 
-Definition unsatisfiable (Gamma:eqns) :=
+
+Definition unsatisfiable (gamma:eqn) :=
+  forall E, ~ satisfies E gamma.
+
+Definition unsatisfiables (Gamma:eqns) :=
   forall E, ~ satisfiesAll E Gamma.
+
+Lemma satisfiesAll_add E gamma Gamma
+  : satisfiesAll E {gamma ; Gamma}
+    <-> satisfies E gamma /\ satisfiesAll E Gamma.
+Proof.
+  split.
+  intros H; split; hnf; intros; eapply H; cset_tac; intuition.
+  intros [A B]; hnf; intros. cset_tac'.
+  destruct H0; dcr; subst; eauto.
+Qed.
+
+Lemma unsatisfiable_add_left gamma Gamma
+  : (forall E, satisfiesAll E Gamma -> ~ satisfies E gamma)
+    -> unsatisfiables {gamma; Gamma}.
+Proof.
+  intros; hnf; intros.
+  intro. eapply satisfiesAll_add in H0; dcr.
+  eapply H; eauto with cset.
+Qed.
+
+Lemma unsatisfiable_monotone Gamma Γ'
+: unsatisfiables Gamma
+  -> Gamma ⊆ Γ'
+  -> unsatisfiables Γ'.
+Proof.
+  intros. hnf; intros. intro. eapply H.
+  eapply satisfiesAll_monotone; eauto.
+Qed.
+
+
+Instance entails_entails_morphism_impl
+: Proper (flip entails ==> entails ==> impl) entails.
+Proof.
+  unfold Proper, respectful, flip, impl, entails; intros; dcr; intros; eauto.
+Qed.
+
+Instance entails_entails_morphism_flip_impl
+: Proper (entails ==> flip entails ==> flip impl) entails.
+Proof.
+  unfold Proper, respectful, flip, impl, entails; intros; dcr; intros; eauto.
+Qed.
+
+
+Lemma entails_subset Γ Γ'
+  : Γ' ⊆ Γ
+    -> entails Γ Γ'.
+Proof.
+  unfold entails, satisfiesAll; intuition.
+Qed.
+
+
+Lemma entails_add Gamma gamma Γ'
+: entails Gamma ({{gamma}} ∪ Γ')
+  -> entails Gamma Γ'.
+Proof.
+  unfold entails; intros; dcr; intros.
+  - hnf; intros. eapply H; eauto. cset_tac; intuition.
+Qed.
+
+Lemma entails_add' Gamma gamma Γ'
+: entails Gamma Γ'
+  -> entails Gamma {{gamma}}
+  -> entails Gamma {gamma; Γ'}.
+Proof.
+  unfold entails; intros; dcr; intros.
+  - hnf; intros. cset_tac'.
+    + eapply H0; cset_tac.
+    + eapply H; eauto.
+Qed.
+
+
+Lemma entails_monotonic_add Gamma Γ' gamma
+: entails Gamma Γ' -> entails (gamma ∪ Gamma) Γ'.
+Proof.
+  unfold entails; intros; dcr.
+  - hnf; intros. eapply H. hnf; intros. eapply H0.
+    cset_tac. eauto.
+Qed.
+
+Lemma entails_union_split Gamma Γ' Γ''
+: entails Gamma (Γ' ∪ Γ'')
+-> entails Gamma (Γ')
+/\ entails Gamma (Γ'').
+Proof.
+  unfold entails, satisfiesAll.
+  split; intros; dcr.
+    + eapply H; eauto. cset_tac; intuition.
+    + eapply H; eauto. cset_tac; intuition.
+Qed.
+
+Lemma entails_union Gamma Γ' Γ''
+: entails Gamma (Γ')
+/\ entails Gamma (Γ'')
+-> entails Gamma (Γ' ∪ Γ'').
+Proof.
+  unfold entails, satisfiesAll.
+  intros; dcr.
+  + intros. cset_tac.
+Qed.
+
+Lemma entails_add_single Gamma gamma Γ'
+  : entails Gamma Γ'
+    -> entails Gamma {gamma}
+    -> entails Gamma {gamma; Γ'}.
+Proof.
+  unfold entails; intros; dcr; intros.
+  - hnf; intros. cset_tac'.
+    + eapply H0; cset_tac.
+    + eapply H; eauto.
+Qed.
+
+Instance satisfiesAll_Subset_morphism
+  : Proper (eq ==> Subset ==> flip impl) satisfiesAll.
+Proof.
+  unfold Proper, respectful, flip, impl; intros; subst.
+  hnf; intros. eapply H1. cset_tac.
+Qed.
+
+Instance satisfiesAll_Equal_morphism
+  : Proper (eq ==> Equal ==> iff) satisfiesAll.
+Proof.
+  unfold Proper, respectful; intros; subst.
+  intuition.
+  - rewrite <- H0; eauto.
+  - rewrite H0; eauto.
+Qed.
+
+
+Lemma entails_monotone Γ1 Γ2 Γ1'
+: entails Γ1 Γ2
+  -> Γ1 ⊆ Γ1'
+  -> entails Γ1' Γ2.
+Proof.
+  unfold entails; intros; dcr.
+  - intros. eapply H. hnf; intros. eapply H1; eauto.
+Qed.
+
+
+Instance entails_morphism_add gamma
+: Proper (entails ==> entails) (add gamma).
+Proof.
+  unfold Proper, respectful; intros.
+  eapply entails_add'.
+  - eapply entails_monotone; cset_tac; eauto.
+  - eapply entails_subset; cset_tac; eauto.
+Qed.
+
+
+
+Instance entails_morphism_impl
+: Proper (Subset ==> flip Subset ==> impl) entails.
+Proof.
+  unfold Proper, respectful, flip, impl, entails, satisfiesAll; intros; dcr; intros.
+  eapply H1; eauto.
+Qed.
+
+Instance entails_morphism_flip_impl
+: Proper (flip Subset ==> Subset ==> flip impl) entails.
+Proof.
+  unfold Proper, respectful, flip, impl, entails, satisfiesAll; intros; dcr; intros.
+  eapply H1; eauto.
+Qed.
+
+
+Instance entails_morphism_impl_iff
+: Proper (Equal ==> Equal ==> iff) entails.
+Proof.
+  unfold Proper, respectful, flip; intros; dcr; split; intros.
+  - eapply entails_morphism_impl; eauto.
+    + rewrite H; reflexivity.
+    + rewrite H0; reflexivity.
+  - eapply entails_morphism_impl; eauto.
+    + rewrite H; reflexivity.
+    + rewrite H0; reflexivity.
+Qed.
+
+Lemma entails_union' Gamma Γ' Γ'' Γ'''
+  : Γ''' ⊆ Γ' ∪ Γ''
+    -> entails Gamma (Γ')
+    -> entails Gamma (Γ'')
+    -> entails Gamma (Γ''').
+Proof.
+  intros; hnf; intros; hnf; intros.
+  rewrite H in H3. cset_tac'.
+  - eapply H0; eauto.
+  - eapply H1; eauto.
+Qed.
+
+Instance entails_refl
+  : Reflexive (entails).
+Proof.
+  hnf; intros. unfold entails; intros; eauto; try reflexivity.
+Qed.
+
+Lemma entails_empty s
+  : entails s ∅.
+Proof.
+  hnf; intros. intros.
+  - hnf; intros. cset_tac; intuition.
+Qed.
+
+Lemma entails_eqns_trans Gamma e e' e''
+  : EqnEq e e' ∈ Gamma
+    -> EqnEq e' e'' ∈ Gamma
+    -> entails Gamma {EqnEq e e''}.
+Proof.
+  intros. hnf; intros.
+  hnf; intros. cset_tac'. hnf; intros. rewrite <- H2.
+  exploit (H1 _ H); eauto.
+  exploit (H1 _ H0); eauto.
+  etransitivity; eauto.
+Qed.
+
+
+Lemma entails_eqns_apx_refl e Gamma
+  : entails Gamma {EqnApx e e}.
+Proof.
+  hnf; intros. hnf; intros. hnf; intros.
+  cset_tac'. rewrite <- H0.
+  reflexivity.
+Qed.
+
+Lemma satisfiesAll_union E Gamma Γ'
+  : satisfiesAll E (Gamma ∪ Γ')
+    <-> satisfiesAll E Gamma /\ satisfiesAll E Γ'.
+Proof.
+  split.
+  intros H; split; hnf; intros; eapply H; cset_tac; intuition.
+  intros [A B]; hnf; intros. cset_tac.
+Qed.
+
+Lemma satisfies_agree E E' gamma
+  : satisfies E gamma
+    -> agree_on eq (freeVars gamma) E E'
+    -> satisfies E' gamma.
+Proof.
+  intros. general induction gamma; simpl in *.
+  - erewrite !op_eval_agree; eauto with cset.
+  - erewrite !op_eval_agree; eauto with cset.
+  - eauto.
+Qed.
+
+Instance subst_eqn_Proper ϱ
+  : Proper (_eq ==> _eq) (subst_eqn ϱ).
+Proof.
+  hnf; intros. invc H. simpl in *; subst. reflexivity.
+Qed.
+
+Instance subst_eqns_morphism
+: Proper (eq ==> Equal ==> Equal) subst_eqns.
+Proof.
+  unfold Proper, respectful, subst_eqns; intros; subst.
+  eapply map_Proper; eauto.
+  hnf; intros; split.
+  reflexivity.
+  split; eauto using subst_eqn_Proper.
+Qed.
+
+Instance subst_eqns_morphism_subset
+: Proper (eq ==> Subset ==> Subset) subst_eqns.
+Proof.
+  unfold Proper, respectful, subst_eqns; intros; subst.
+  rewrite H0. reflexivity.
+Qed.
+
+Instance subst_eqns_morphism_subset_flip
+: Proper (eq ==> flip Subset ==> flip Subset) subst_eqns.
+Proof.
+  unfold Proper, respectful, subst_eqns; intros; subst.
+  rewrite H0. reflexivity.
+Qed.
+
+Lemma in_subst_eqns (Gamma:eqns) ϱ gamma
+  : gamma ∈ Gamma
+    -> subst_eqn ϱ gamma ∈ subst_eqns ϱ Gamma.
+Proof.
+  intros. unfold subst_eqns.
+  eapply map_1; eauto. intuition.
+Qed.
+
+
+Instance exp_freeVars_Proper
+  :  Proper (eq ==> Equal) Exp.freeVars.
+Proof.
+  unfold Proper, respectful; intros.
+  inv H. general induction y; simpl; hnf; intuition.
+Qed.
+
+Instance freeVars_Proper
+  :  Proper (_eq ==> _eq) freeVars.
+Proof.
+  hnf; intros. inv H. reflexivity.
+Qed.
+
+Lemma eqns_freeVars_incl (Gamma:eqns) gamma
+  : gamma ∈ Gamma
+    -> freeVars gamma ⊆ eqns_freeVars Gamma.
+Proof.
+  intros. unfold eqns_freeVars.
+  hnf; intros. eapply fold_union_incl; eauto.
+  eapply map_1; eauto. eapply freeVars_Proper.
+Qed.
+
+Hint Resolve eqns_freeVars_incl : cset.
+
+Lemma satisfiesAll_agree E E' Gamma
+  : satisfiesAll E Gamma
+    -> agree_on eq (eqns_freeVars Gamma) E E'
+    -> satisfiesAll E' Gamma.
+Proof.
+  intros; hnf; intros.
+  eapply satisfies_agree; eauto.
+  eapply agree_on_incl; eauto with cset.
+Qed.
+
+Lemma satisfies_update_dead E gamma x v
+: satisfies E gamma
+  -> x ∉ freeVars gamma
+  -> satisfies (E[x <- v]) gamma.
+Proof.
+  intros.
+  eapply satisfies_agree; eauto.
+  symmetry.
+  eapply agree_on_update_dead; eauto.
+Qed.
+
+
+Lemma entails_inert Γ1 Γ2 Γ2'
+: entails Γ2 Γ2'
+  -> entails (Γ1 ∪ Γ2) (Γ1 ∪ Γ2').
+Proof.
+  unfold entails; intros; dcr.
+  - eapply satisfiesAll_union.
+    eapply satisfiesAll_union in H0.
+    dcr; split; eauto.
+Qed.
+
+Lemma entails_inert_add x Γ2 Γ2'
+  : entails Γ2 Γ2'
+    -> entails {x ; Γ2} {x ; Γ2'}.
+Proof.
+  unfold entails; intros; dcr.
+  - hnf; intros. cset_tac'.
+    + eapply H0. cset_tac.
+    + eapply H; eauto. hnf; intros; eapply H0.
+      cset_tac.
+Qed.
+
+Lemma entails_transitive Γ Γ' Γ''
+  : entails Γ Γ' -> entails Γ' Γ'' -> entails Γ Γ''.
+Proof.
+  intros; hnf; intros.
+  - eapply H0; eauto.
+Qed.
+
+Instance entails_trans : Transitive entails.
+Proof.
+  hnf.
+  eapply entails_transitive.
+Qed.
+
+Lemma not_entails_entails_antitone Gamma Γ' gamma
+  : not_entails Γ' gamma
+    -> entails Γ' Gamma
+    -> not_entails Gamma gamma.
+Proof.
+  intros. hnf; intros.
+  edestruct H as [E ?]; dcr.
+  eexists E; intros; split; eauto.
+Qed.
+
+Lemma unsatisfiable_entails_monotone Gamma Γ'
+  : unsatisfiables Gamma
+    -> entails Γ' Gamma
+    -> unsatisfiables Γ'.
+Proof.
+  intros. hnf; intros. intro. exploit (H E); eauto.
+Qed.
+
+
+Lemma satisfies_fstNoneOrR_apx V e e' :
+  satisfies V (EqnApx e e') -> fstNoneOrR eq (op_eval V e) (op_eval V e').
+Proof.
+  intros. eauto.
+Qed.
+
+Lemma onvLe_op_eval_some V V'
+  :onvLe V V' -> forall e v, op_eval V e = ⎣ v ⎦ -> op_eval V' e = ⎣ v ⎦.
+Proof.
+  intros. general induction e; simpl in * |- * ; eauto using @fstNoneOrR.
+  - rewrite H0. exploit H; eauto.
+  - monad_inv H0. rewrite EQ. simpl. erewrite (IHe V V' H _ EQ); eauto.
+  - monad_inv H0. rewrite EQ1. rewrite EQ. simpl.
+    erewrite IHe1; eauto. erewrite IHe2; simpl; eauto.
+Qed.
+
+
+Lemma onvLe_fstNoneOrR_apx V V' e :
+  onvLe V V' -> fstNoneOrR eq (op_eval V e) (op_eval V' e).
+Proof with simpl; eauto using @fstNoneOrR, @onvLe_op_eval_some.
+  intros. case_eq (op_eval V e) ...
+  intros. erewrite onvLe_op_eval_some...
+Qed.
+
+Lemma satisfies_EqnEq_on_update   (x:var) e V v:
+  op_eval V e = ⎣ v ⎦   -> x ∉ Op.freeVars e  ->satisfies (V [x <- ⎣ v ⎦]) (EqnEq(Var x) e).
+Proof.
+  intros. unfold satisfies. simpl. lud; eauto.
+    erewrite op_eval_live.
+    -  rewrite <- H. reflexivity.
+    - eapply Op.live_freeVars.
+    - eapply agree_on_update_dead; eauto.
+Qed.
+
+
+
+Lemma op_eval_true_satisfies  V e v
+        : op_eval V e = ⎣ v ⎦ -> val2bool v = true -> satisfies V (EqnEq (UnOp UnOpToBool e) (Con val_true)).
+Proof.
+  intros. unfold satisfies. simpl. rewrite H. simpl. unfold option_lift1. rewrite H0. simpl. reflexivity.
+Qed.
+
+Lemma op_eval_false_satisfies V e v
+  : op_eval V e = ⎣ v ⎦ -> val2bool v = false -> satisfies V (EqnEq (UnOp UnOpToBool e) (Con val_false)).
+Proof.
+intros.  unfold satisfies. simpl. rewrite H. simpl. unfold option_lift1. rewrite H0. simpl. reflexivity.
+Qed.
+
+Lemma onvLe_omap_op_eval_some V V' Y vl
+ : onvLe V V' -> (omap (op_eval V) Y) = ⎣ vl ⎦ -> (omap (op_eval V') Y) = ⎣ vl ⎦.
+Proof.
+  intros.
+  general induction Y; simpl in * |- *; eauto.
+  monad_inv H0.
+  rewrite EQ, EQ1. simpl.
+  exploit (onvLe_op_eval_some H) as EV; eauto. rewrite EV.
+  simpl. erewrite IHY; eauto.
+  reflexivity.
+Qed.
+
+Lemma onvLe_omap_op_eval_fstNoneOrEq V V' Y
+  : onvLe V V'
+    -> fstNoneOrR eq (omap (op_eval V) Y) (omap (op_eval V') Y).
+Proof.
+  intros.
+  case_eq (omap (op_eval V) Y); eauto using @fstNoneOrR.
+  intros. exploit onvLe_omap_op_eval_some  ; eauto. rewrite H1.
+  reflexivity.
+Qed.
+
+Lemma omap_satisfies_list_EqnApx V Y Y' v
+  : length Y = length Y'
+    -> satisfiesAll V (list_EqnApx Y Y')
+    -> omap (op_eval V) Y = ⎣ v ⎦
+    -> omap (op_eval V) Y' = ⎣ v ⎦.
+Proof.
+  intros. length_equify.
+  general induction H; simpl in * |- *; eauto.
+  monad_inv H1.
+  exploit H0. eapply add_1. reflexivity. inv H1. congruence.
+  simpl. erewrite IHlength_eq; eauto. rewrite EQ1. reflexivity.
+  eapply satisfiesAll_monotone; eauto.
+  unfold list_EqnApx; simpl in *.
+  cset_tac; intuition.
+Qed.
+
+Lemma satisfies_omap_op_eval_fstNoneOrR V Y Y'
+  : ❬Y❭ = ❬Y'❭
+    -> satisfiesAll V (list_EqnApx Y Y')
+    -> fstNoneOrR eq (omap (op_eval V) Y) (omap (op_eval V) Y').
+Proof.
+  intros.
+  case_eq (omap (op_eval V) Y); eauto using fstNoneOrR.
+  intros. length_equify.
+  erewrite (@omap_satisfies_list_EqnApx V Y Y' l ) ; eauto using length_eq_length, fstNoneOrR.
+Qed.
+
+Lemma onvLe_op_eval_satisfies V V' e e' v
+  : onvLe V V'
+    -> op_eval V e = Some v
+    -> satisfies V (EqnApx e e')
+    -> satisfies V' (EqnApx e e').
+Proof.
+  intros.
+  unfold satisfies in *. rewrite H0 in H1. inv H1.
+  symmetry in H3. eapply onvLe_op_eval_some in H3; eauto. eapply onvLe_op_eval_some in H0; eauto.
+  rewrite H0,H3. reflexivity.
+Qed.
+
+Lemma onvLe_op_eval_satisfiesAll V V' Y Y' v
+  : onvLe V V'
+    -> ❬Y❭ = ❬Y'❭
+    -> (omap (op_eval V) Y) = Some v
+    -> satisfiesAll V (list_EqnApx Y Y')
+    -> satisfiesAll V' (list_EqnApx Y Y').
+Proof.
+  intros.
+  unfold satisfiesAll in *. intros.
+  length_equify. general induction H0; simpl in * |- *;  eauto.
+  - unfold list_EqnApx in H3. simpl in *. cset_tac.
+  - unfold list_EqnApx in *. simpl in * |- *.
+    cset_tac'.
+    + monad_inv H1. rewrite <- H5. eapply onvLe_op_eval_satisfies; eauto.
+    + monad_inv H1. eapply IHlength_eq; eauto.
+Qed.
+
+
+Lemma in_eqns_freeVars x gamma Gamma
+  : x \In freeVars gamma
+    -> gamma ∈ Gamma
+    -> x \In eqns_freeVars Gamma.
+Proof.
+  intros. eapply eqns_freeVars_incl; eauto.
+Qed.
+
+Lemma satisfiesAll_EqnEq_on_update V v x Gamma
+  : satisfiesAll V Gamma
+    -> x ∉ eqns_freeVars Gamma
+    -> satisfiesAll (V [x <- ⎣ v ⎦] ) Gamma.
+Proof.
+  intros.
+  unfold satisfiesAll in *.
+  intros.
+  eapply satisfies_update_dead; eauto.
+  intros A. eapply H0. eapply in_eqns_freeVars; eauto.
+Qed.
+
+Lemma omap_exp_eval_onvLe Y E E' v
+  : onvLe E E'
+    -> omap (op_eval E) Y = Some v
+    -> omap (op_eval E') Y = Some v.
+Proof.
+  intros. general induction Y; simpl in * |- *; eauto.
+  simpl in H0. rewrite H0.
+  monad_inv H0.
+  erewrite exp_eval_onvLe; try eapply H; eauto. simpl.
+  erewrite IHY; eauto; simpl; eauto.
+Qed.
+
+
+
+Lemma eqns_freeVars_union Gamma Γ'
+  : eqns_freeVars (Gamma ∪ Γ') [=] eqns_freeVars (Gamma) ∪ eqns_freeVars Γ'.
+Proof.
+  unfold eqns_freeVars.
+  rewrite map_app; eauto using freeVars_Proper.
+  rewrite fold_union_app. reflexivity.
+Qed.
+
+Lemma fold_union_add X `{OrderedType X} x Γ
+: fold union ({x; Γ}) {}[=]
+  x ∪ fold union Γ {}.
+Proof.
+  assert ({x; Γ} [=] {{x}} ∪ Γ).
+  cset_tac; intuition. rewrite H0.
+  rewrite fold_union_app.
+  rewrite fold_single; eauto using Equal_ST, union_m, transpose_union.
+  clear; cset_tac.
+Qed.
+
+Lemma eqns_freeVars_add Gamma e
+  : eqns_freeVars {e; Gamma} [=] eqns_freeVars (Gamma) ∪ freeVars e.
+Proof.
+  intros. unfold eqns_freeVars.
+  rewrite map_add; eauto using freeVars_Proper.
+  rewrite fold_union_add.
+  cset_tac.
+Qed.
+
+Lemma eqns_freeVars_add2 Gamma e e'
+  : eqns_freeVars ({e; { e'; Gamma } }) [=] eqns_freeVars (Gamma) ∪ freeVars e ∪ freeVars e'.
+Proof.
+  intros. unfold eqns_freeVars.
+  repeat rewrite map_add; eauto using freeVars_Proper.
+  repeat rewrite fold_union_add.
+  cset_tac.
+Qed.
+
+Lemma eqns_freeVars_add' Gamma e
+  : eqns_freeVars ({e ; Gamma}) [=] eqns_freeVars (Gamma) ∪ freeVars e.
+Proof.
+  intros. unfold eqns_freeVars.
+  rewrite map_add, fold_union_add.
+  cset_tac; intuition. intuition.
+Qed.
+
+
+Instance map_freeVars_morphism
+: Proper (Subset ==> Subset) (map freeVars).
+Proof.
+  unfold Proper, respectful; intros.
+  hnf; intros. eapply map_iff; eauto using freeVars_Proper.
+  eapply map_iff in H0; eauto using freeVars_Proper.
+  destruct H0; dcr. eexists x0; split; eauto.
+Qed.
+
+Instance eqns_freeVars_morphism
+: Proper (Subset ==> Subset) eqns_freeVars.
+Proof.
+  unfold Proper, respectful, eqns_freeVars; intros.
+  rewrite H. reflexivity.
+Qed.
+
+Instance eqns_freeVars_morphism_flip
+: Proper (flip Subset ==> flip Subset) eqns_freeVars.
+Proof.
+  unfold Proper, respectful, eqns_freeVars, flip; intros.
+  rewrite H. reflexivity.
+Qed.
+
+Instance eqns_freeVars_morphism_equal
+: Proper (Equal ==> Equal) eqns_freeVars.
+Proof.
+  unfold Proper, respectful, eqns_freeVars, flip; intros.
+  rewrite H. reflexivity.
+Qed.
+
+
+
+Lemma agree_on_onvLe X (V V': onv X) x v
+  :onvLe V V'
+         -> onvLe (V [x <- v]) (V' [x <- v]).
+Proof.
+  intros. hnf. intros.
+  decide (x0 = x).
+  - subst. lud. eauto.
+  - lud. eapply H. eauto.
+Qed.
+
+
+
+Lemma agree_on_onvLe_update_list {X} `{OrderedType.OrderedType X} (V V':onv X) Z vl
+: onvLe V V'
+  -> onvLe (V [Z <-- vl]) (V' [Z <-- vl]).
+Proof.
+  intros; hnf; intros.
+  decide (x ∈ of_list Z).
+  - general induction Z; simpl in * |- *; eauto.
+    + cset_tac; intuition.
+    + destruct vl.
+      * rewrite H1. eapply H0 in H1. eauto.
+      * lud. erewrite IHZ; eauto. cset_tac; intuition.
+  - rewrite lookup_set_update_not_in_Z; eauto.
+    rewrite lookup_set_update_not_in_Z in H1; eauto.
+Qed.
+
+Instance unsatisfiables_Proper_impl
+  : Proper (Subset ==> impl) unsatisfiables.
+Proof.
+  unfold Proper, respectful, flip, impl; intros.
+  hnf; intros. rewrite <- H. eauto.
+Qed.
+
+Instance unsatisfiables_Proper_iff
+  : Proper (Equal ==> iff) unsatisfiables.
+Proof.
+  unfold Proper, respectful, flip, impl; intros.
+  intuition; eapply unsatisfiables_Proper_impl; eauto;
+    rewrite H; eauto.
+Qed.
